tests/Sum_ContractAction.bpl
@@ -1,0 +1,68 @@
+// ---------------------------------------------------------------
+// -- Types and global variables ---------------------------------
+// ---------------------------------------------------------------
+type Ref;
+type Chan a;
+type Field a;
+type Actor;
+type CType = <a>[Chan a]int;
+type MType = <a>[Chan a][int]a;
+type Obj = <a>[Field a]a;
+type HType = [Ref]Obj;
+
+var M: MType;
+var C: CType;
+var R: CType;
+var I: CType;
+var B: CType;
+
+var H: HType;
+
+const unique this#: Actor;
+
+function AT#Min(x:int, y: int): int { if x <= y then x else y }
+function AT#Ite<T>(bool, T, T): T;
+axiom (
+  forall<T> cond: bool, thn: T, els: T :: { AT#Ite(cond, thn, els) }
+    (cond ==> AT#Ite(cond,thn,els) == thn &&
+    !cond ==> AT#Ite(cond,thn,els) == els)
+);
+
+// ---------------------------------------------------------------
+// -- End of prelude ---------------------------------------------
+// ---------------------------------------------------------------
+
+procedure Sum#init#0()
+  modifies C, R, M, I, H;
+{
+  var x: Chan (int);
+  var y: Chan (int);
+  var Ch#sum: Chan (int);
+  var sum: int;
+  assume x != y;
+  assume R[x] == 0;
+  assume C[y] == 0;
+  assume (R[Ch#sum] == 0) && (C[Ch#sum] == 0);
+  sum := 0;
+}
+procedure Sum#anon$1#1()
+  modifies C, R, M, I, H;
+{
+  var x: Chan (int);
+  var y: Chan (int);
+  var Ch#sum: Chan (int);
+  var sum: int;
+  var x#0: int;
+  assume x != y;
+  assume 0 <= R[x];
+  assume 0 <= C[y];
+  assume (0 <= R[Ch#sum]) && (C[Ch#sum] == (R[Ch#sum] + 1));
+  assume R[x] == C[y];
+  x#0 := M[x][R[x]];
+  R[x] := R[x] + 1;
+  assume 0 <= x#0;
+  sum := sum + x#0;
+  assert {:msg "Sum_ContractAction.actor(17.13): Action postcondition might not hold (#0)"} x#0 <= sum;
+  M[y][C[y]] := sum;
+  C[y] := C[y] + 1;
+}
